BPlusTree_Range.thy
@@ -1,25 +1,26 @@
 theory BPlusTree_Range
 imports BPlusTree
     "HOL-Data_Structures.Set_Specs"
+    BPlusTree_Set
 begin
 
-definition lower_bound where
-  "lower_bound y X = Min ({x \<in> X. x \<ge> y} \<union> {top})"
+definition Lower_bound where
+  "Lower_bound y X = Min ({x \<in> X. x \<ge> y} \<union> {top})"
 
 
-fun lower_bound_list where
-"lower_bound_list (y::'a::{linorder, order_top}) (x#xs) = (if x \<ge> y then x else lower_bound_list y xs)" |
-"lower_bound_list y [] = top"
+fun lower_bound where
+"lower_bound (y::'a::{linorder, order_top}) (x#xs) = (if x \<ge> y then x else lower_bound y xs)" |
+"lower_bound y [] = top"
 
-lemma lower_bound_empty: "lower_bound y {} = top"
-  unfolding lower_bound_def
+lemma Lower_bound_empty: "Lower_bound y {} = top"
+  unfolding Lower_bound_def
   by auto
 
-lemma lower_bound_list_set: "sorted_less xs \<Longrightarrow>
-  lower_bound_list y xs = lower_bound y (set xs)"
+lemma lower_bound_set: "sorted_less xs \<Longrightarrow>
+  lower_bound y xs = Lower_bound y (set xs)"
 proof(induction xs)
   case Nil
-  then show ?case by (auto simp add: lower_bound_def)
+  then show ?case by (auto simp add: Lower_bound_def)
 next
 case (Cons x xs)
   then show ?case 
@@ -29,15 +30,15 @@ case (Cons x xs)
       using Cons.prems True by auto
     then have "{xa \<in> set (x # xs). y \<le> xa} = set(x#xs)"
       by auto
-    then have "lower_bound y (set (x#xs)) = Min (set (x#xs) \<union> {top})"
-      unfolding lower_bound_def
+    then have "Lower_bound y (set (x#xs)) = Min (set (x#xs) \<union> {top})"
+      unfolding Lower_bound_def
       by auto
     moreover have "x = Min (set (x#xs) \<union> {top})"
       using Cons.prems
       by (metis List.finite_set Min.union Min_insert2 Min_singleton less_imp_le list.simps(15) list.simps(3) min_def set_empty sorted_Cons_iff top_greatest)
     ultimately show ?thesis 
       using Cons.prems True
-      by (auto simp add: lower_bound_def)
+      by (auto simp add: Lower_bound_def)
   next
     case False
     then have "{xa \<in> set (x # xs). y \<le> xa} = {xa \<in> set xs. y \<le> xa}"
@@ -46,13 +47,13 @@ case (Cons x xs)
       using Cons.prems by auto
     ultimately show ?thesis
       using False Cons.IH
-      by (simp add: lower_bound_def)
+      by (simp add: Lower_bound_def)
   qed
 qed
 
 lemma lower_bound_split: "sorted_less (xs@x#ys) \<Longrightarrow>
-  lower_bound_list y (xs@x#ys) =
-  (if x < y then lower_bound_list y ys else lower_bound_list y (xs@[x]))" 
+  lower_bound y (xs@x#ys) =
+  (if x < y then lower_bound y ys else lower_bound y (xs@[x]))" 
   apply (induction xs) 
   apply auto
   done
@@ -61,43 +62,43 @@ lemma lower_bound_split: "sorted_less (xs@x#ys) \<Longrightarrow>
    we need to find a different value with similar properties
    compatible with the current tree structure *)
 
-definition lower_bound2 where
-  "lower_bound2 y X = Max ({x \<in> X. x < y} \<union> {bot})"
+definition Lower_bound2 where
+  "Lower_bound2 y X = Max ({x \<in> X. x < y} \<union> {bot})"
 
 
-fun lower_bound2_list where
-"lower_bound2_list (y::'a::{linorder, order_bot}) (x#xs) = (if (last (x#xs)) < y then (last (x#xs)) else lower_bound2_list y (butlast (x#xs)))" |
-"lower_bound2_list y [] = bot"
+fun lower_bound2 where
+"lower_bound2 (y::'a::{linorder, order_bot}) (x#xs) = (if (last (x#xs)) < y then (last (x#xs)) else lower_bound2 y (butlast (x#xs)))" |
+"lower_bound2 y [] = bot"
 
-declare lower_bound2_list.simps[simp del]
+declare lower_bound2.simps[simp del]
 
-lemma lower_bound2_list_simps [simp]:
-  "lower_bound2_list y (xs@[x]) = (if x < y then x else lower_bound2_list y xs)"
-  "lower_bound2_list y [] = bot"
+lemma lower_bound2_simps [simp]:
+  "lower_bound2 y (xs@[x]) = (if x < y then x else lower_bound2 y xs)"
+  "lower_bound2 y [] = bot"
 proof (goal_cases)
   case 1
   obtain xs' x' where *: "xs@[x] = x'#xs'"
     by (metis Nil_is_append_conv neq_Nil_conv)
   show ?case
     apply(subst *)+
-    apply(subst lower_bound2_list.simps)
+    apply(subst lower_bound2.simps)
     apply(subst *[symmetric])+
     apply auto
     done
-qed (auto simp add: lower_bound2_list.simps)
+qed (auto simp add: lower_bound2.simps)
 
 
 
-lemma lower_bound2_empty: "lower_bound2 y {} = bot"
-  unfolding lower_bound2_def
+lemma Lower_bound2_empty: "Lower_bound2 y {} = bot"
+  unfolding Lower_bound2_def
   by auto
 
 
-lemma lower_bound2_list_set: "sorted_less xs \<Longrightarrow>
-  lower_bound2_list y xs = lower_bound2 y (set xs)"
+lemma lower_bound2_set: "sorted_less xs \<Longrightarrow>
+  lower_bound2 y xs = Lower_bound2 y (set xs)"
 proof(induction xs rule: rev_induct)
   case Nil
-  then show ?case by (auto simp add: lower_bound2_def)
+  then show ?case by (auto simp add: Lower_bound2_def)
 next
   case (snoc x xs)
   then obtain x' xs' where *: "x'#xs' = xs@[x]"
@@ -110,15 +111,15 @@ next
       by (auto simp add: sorted_snoc_iff)
     then have "{xa \<in> set (xs@[x]). xa < y} = set(xs@[x])"
       by auto
-    then have "lower_bound2 y (set (xs@[x])) = Max (set (xs@[x]) \<union> {bot})"
-      unfolding lower_bound2_def
+    then have "Lower_bound2 y (set (xs@[x])) = Max (set (xs@[x]) \<union> {bot})"
+      unfolding Lower_bound2_def
       by auto
     moreover have "x = Max (set (xs@[x]) \<union> {bot})"
       using snoc.prems
       by (auto simp add: Max_insert2 less_imp_le sorted_snoc_iff)
     ultimately show ?thesis 
       using snoc.prems True
-      by (auto simp add: lower_bound2_def sorted_snoc_iff)
+      by (auto simp add: Lower_bound2_def sorted_snoc_iff)
   next
     case False
     then have "{xa \<in> set (xs@[x]). xa < y} = {xa \<in> set xs. xa < y}"
@@ -127,20 +128,20 @@ next
       using snoc.prems sorted_snoc_iff by auto
     ultimately show ?thesis
       using False snoc.IH
-      by (simp add: lower_bound2_def)
+      by (simp add: Lower_bound2_def)
   qed
 qed
 
 lemma lower_bound2_split: "sorted_less (xs@x#ys) \<Longrightarrow>
-  lower_bound2_list y (xs@x#ys) =
-  (if x < y then lower_bound2_list y (x#ys) else lower_bound2_list y xs)" 
+  lower_bound2 y (xs@x#ys) =
+  (if x < y then lower_bound2 y (x#ys) else lower_bound2 y xs)" 
   apply(induction ys rule: rev_induct)
-  subgoal by (simp add: lower_bound2_list.simps(1))
+  subgoal by (simp add: lower_bound2.simps(1))
   apply (auto)
   subgoal for x' xs'
-    by (smt (verit, del_insts) Nil_is_append_conv butlast.simps(2) butlast_append butlast_snoc last_appendR list.distinct(1) lower_bound2_list.elims sorted_mid_iff sorted_mid_iff2)
+    by (smt (verit, del_insts) Nil_is_append_conv butlast.simps(2) butlast_append butlast_snoc last_appendR list.distinct(1) lower_bound2.elims sorted_mid_iff sorted_mid_iff2)
   subgoal for x' xs'
-    by (smt (verit, ccfv_threshold) Nil_is_append_conv butlast.simps(2) butlast_append butlast_snoc dual_order.strict_trans last.simps last_appendR last_snoc lower_bound2_list.elims sorted_mid_iff sorted_mid_iff2)
+    by (smt (verit, ccfv_threshold) Nil_is_append_conv butlast.simps(2) butlast_append butlast_snoc dual_order.strict_trans last.simps last_appendR last_snoc lower_bound2.elims sorted_mid_iff sorted_mid_iff2)
   done
 
 
@@ -148,18 +149,18 @@ lemma lower_bound2_split: "sorted_less (xs@x#ys) \<Longrightarrow>
 in the sorted list.
 in other words there is no element between them.
 in other words all elements are smeq or greq. *)
-lemma lower_bound_12_neighbours:
+lemma Lower_bound_12_neighbours:
   assumes "finite X"
-  shows "\<forall>x \<in> X. x \<le> lower_bound2 y X \<or> lower_bound y X \<le> x"
+  shows "\<forall>x \<in> X. x \<le> Lower_bound2 y X \<or> Lower_bound y X \<le> x"
 proof (standard, goal_cases)
   case (1 x)
-  have "\<not>(x > lower_bound2 y X \<and> x < lower_bound y X)"
+  have "\<not>(x > Lower_bound2 y X \<and> x < Lower_bound y X)"
   proof (rule ccontr, goal_cases)
     case contr: 1
-    then have "x > lower_bound2 y X"
+    then have "x > Lower_bound2 y X"
       by auto
     then have **: "x \<ge> y"
-      unfolding lower_bound2_def
+      unfolding Lower_bound2_def
     proof(cases "x < y")
       case True
       then have *: "x \<in> {x \<in> X. x < y}"
@@ -168,16 +169,16 @@ proof (standard, goal_cases)
         using assms by auto
       ultimately have "x \<le> Max {x \<in> X. x < y}"
         using Max.coboundedI by blast
-      then have "x \<le> lower_bound2 y X"
-        unfolding lower_bound2_def
+      then have "x \<le> Lower_bound2 y X"
+        unfolding Lower_bound2_def
         using "*" \<open>finite {x \<in> X. x < y}\<close> by auto
       then show ?thesis
-        using \<open>lower_bound2 y X < x\<close> by auto
+        using \<open>Lower_bound2 y X < x\<close> by auto
     qed simp
-    from contr have "x < lower_bound y X"
+    from contr have "x < Lower_bound y X"
       by auto
     then have "x < y"
-      unfolding lower_bound2_def
+      unfolding Lower_bound2_def
     proof(cases "x \<ge> y")
       case True
       then have *: "x \<in> {x \<in> X. x \<ge> y}"
@@ -186,11 +187,11 @@ proof (standard, goal_cases)
         using assms by auto
       ultimately have "x \<ge> Min {x \<in> X. x \<ge> y}"
         using Min.coboundedI by blast
-      then have "x \<ge> lower_bound y X"
-        unfolding lower_bound_def
+      then have "x \<ge> Lower_bound y X"
+        unfolding Lower_bound_def
         using "*" \<open>finite {x \<in> X. x \<ge> y}\<close> by auto
       then show ?thesis
-        using \<open>lower_bound y X > x\<close> by auto
+        using \<open>Lower_bound y X > x\<close> by auto
     qed simp
     then show ?case
       using ** by simp
@@ -199,107 +200,107 @@ proof (standard, goal_cases)
     by auto
 qed
 
-lemma lower_bound_in_X: "finite X \<Longrightarrow> lower_bound y X \<in> X \<union> {top}"
+lemma Lower_bound_in_X: "finite X \<Longrightarrow> Lower_bound y X \<in> X \<union> {top}"
 proof(goal_cases)
   case 1
   have "{x \<in> X. y \<le> x} \<union> {top} \<noteq> {}"
     by auto
   moreover have "finite ({x \<in> X. y \<le> x} \<union> {top})"
     using 1 by auto
-  ultimately have "lower_bound y X \<in> {x \<in> X. y \<le> x} \<union> {top}"
-    unfolding lower_bound_def
+  ultimately have "Lower_bound y X \<in> {x \<in> X. y \<le> x} \<union> {top}"
+    unfolding Lower_bound_def
     using Min_in[of "{x \<in> X. y \<le> x} \<union> {top}"] by blast
   then show ?case
     by blast
 qed
 
-lemma lower_bound2_in_X: "finite X \<Longrightarrow> lower_bound2 y X \<in> X \<union> {bot}"
+lemma Lower_bound2_in_X: "finite X \<Longrightarrow> Lower_bound2 y X \<in> X \<union> {bot}"
 proof(goal_cases)
   case 1
   have "{x \<in> X. y > x} \<union> {bot} \<noteq> {}"
     by auto
   moreover have "finite ({x \<in> X. y > x} \<union> {bot})"
     using 1 by auto
-  ultimately have "lower_bound2 y X \<in> {x \<in> X. y > x} \<union> {bot}"
-    unfolding lower_bound2_def
+  ultimately have "Lower_bound2 y X \<in> {x \<in> X. y > x} \<union> {bot}"
+    unfolding Lower_bound2_def
     using Max_in[of "{x \<in> X. y > x} \<union> {bot}"] by blast
   then show ?case
     by blast
 qed
 
-lemma lb2_le: "finite X \<Longrightarrow> lower_bound2 (y::'a::{linorder,order_bot}) X \<le> y"
+lemma lb2_le: "finite X \<Longrightarrow> Lower_bound2 (y::'a::{linorder,order_bot}) X \<le> y"
 proof(goal_cases)
   case 1
   have "{x \<in> X. y > x} \<union> {bot} \<noteq> {}"
     by auto
   moreover have "finite ({x \<in> X. y > x} \<union> {bot})"
     using 1 by auto
-  ultimately have "lower_bound2 y X \<in> {x \<in> X. y > x} \<union> {bot}"
-    unfolding lower_bound2_def
+  ultimately have "Lower_bound2 y X \<in> {x \<in> X. y > x} \<union> {bot}"
+    unfolding Lower_bound2_def
     using Max_in[of "{x \<in> X. y > x} \<union> {bot}"] by blast
   then show ?case
   proof(standard, goal_cases)
     case 1
-    then have "lower_bound2 y X < y"
+    then have "Lower_bound2 y X < y"
       by blast
     then show ?case
       by simp
   next
     case 2
-    then have "lower_bound2 y X = bot"
+    then have "Lower_bound2 y X = bot"
       by simp
     then show ?case 
       by simp
   qed
 qed
 
-lemma lb_ge: "finite X \<Longrightarrow> lower_bound (y::'a::{linorder,order_top}) X \<ge> y"
+lemma lb_ge: "finite X \<Longrightarrow> Lower_bound (y::'a::{linorder,order_top}) X \<ge> y"
 proof(goal_cases)
   case 1
   have "{x \<in> X. y \<le> x} \<union> {top} \<noteq> {}"
     by auto
   moreover have "finite ({x \<in> X. y \<le> x} \<union> {top})"
     using 1 by auto
-  ultimately have "lower_bound y X \<in> {x \<in> X. y \<le> x} \<union> {top}"
-    unfolding lower_bound_def
+  ultimately have "Lower_bound y X \<in> {x \<in> X. y \<le> x} \<union> {top}"
+    unfolding Lower_bound_def
     using Min_in[of "{x \<in> X. y \<le> x} \<union> {top}"] by blast
   then show ?case
   proof(standard, goal_cases)
     case 1
-    then have "lower_bound y X \<ge> y"
+    then have "Lower_bound y X \<ge> y"
       by blast
     then show ?case
       by simp
   next
     case 2
-    then have "lower_bound y X = top"
+    then have "Lower_bound y X = top"
       by simp
     then show ?case 
       by simp
   qed
 qed
 
-lemma lb2_le_lb: "finite X \<Longrightarrow> lower_bound2 (y::'a::{linorder, order_top,order_bot}) X \<le> lower_bound y X"
+lemma lb2_le_lb: "finite X \<Longrightarrow> Lower_bound2 (y::'a::{linorder, order_top,order_bot}) X \<le> Lower_bound y X"
   by (meson lb2_le lb_ge order_trans)
 
-(* the below lemmata describe how to obtain lower_bound
-once we obtained lower_bound2 - it can be done within constant time! *)
+(* the below lemmata describe how to obtain Lower_bound
+once we obtained Lower_bound2 - it can be done within constant time! *)
 
-lemma "sorted_less (xs@x#y#ys) \<Longrightarrow> x \<noteq> z \<Longrightarrow> x = lower_bound2_list z (xs@x#y#ys) \<Longrightarrow> y = lower_bound_list z (xs@x#y#ys)"
+lemma lb2_obtain_lb: "sorted_less (xs@x#y#ys) \<Longrightarrow> x \<noteq> z \<Longrightarrow> x = lower_bound2 z (xs@x#y#ys) \<Longrightarrow> y = lower_bound z (xs@x#y#ys)"
 proof(goal_cases)
   case assms: 1
-  then have "x = lower_bound2 z (set (xs@x#y#ys))"
-    using lower_bound2_list_set by fastforce
+  then have "x = Lower_bound2 z (set (xs@x#y#ys))"
+    using lower_bound2_set by fastforce
   then have "x < z \<or> x = z"
     by (metis List.finite_set lb2_le order.not_eq_order_implies_strict)
   then show ?thesis
   proof(standard, goal_cases)
     case 1
-    then have "lower_bound_list z (xs@x#y#ys) = lower_bound_list z (y#ys)"
+    then have "lower_bound z (xs@x#y#ys) = lower_bound z (y#ys)"
       using assms lower_bound_split[of xs x "y#ys"]
       by simp
     moreover have "y \<ge> z"
-      by (metis List.finite_set Un_insert_right \<open>x = lower_bound2 z (set (xs @ x # y # ys))\<close> assms(1) insertCI lb_ge list.set(2) lower_bound_12_neighbours not_le order_trans set_append sorted_Cons_iff sorted_wrt_append)
+      by (metis List.finite_set Un_insert_right \<open>x = Lower_bound2 z (set (xs @ x # y # ys))\<close> assms(1) insertCI lb_ge list.set(2) Lower_bound_12_neighbours not_le order_trans set_append sorted_Cons_iff sorted_wrt_append)
     ultimately show ?case
       by simp
   next
@@ -309,11 +310,11 @@ proof(goal_cases)
   qed
 qed
 
-lemma "sorted_less (xs@x#ys) \<Longrightarrow> x = z \<Longrightarrow> x = lower_bound2_list z (xs@x#ys) \<Longrightarrow> x = lower_bound_list z (xs@x#ys)"
+lemma lb2_obtain_lb_edge: "sorted_less (xs@x#ys) \<Longrightarrow> x = z \<Longrightarrow> x = lower_bound2 z (xs@x#ys) \<Longrightarrow> x = lower_bound z (xs@x#ys)"
 proof(goal_cases)
   case assms: 1
-  then have "x = lower_bound2 z (set (xs@x#ys))"
-    using lower_bound2_list_set by fastforce
+  then have "x = Lower_bound2 z (set (xs@x#ys))"
+    using lower_bound2_set by fastforce
   then have "x < z \<or> x = z"
     by (metis List.finite_set lb2_le order.not_eq_order_implies_strict)
   then show ?thesis
@@ -324,12 +325,244 @@ proof(goal_cases)
   next
     case 2
     then have "xs = []"
-      by (metis "2" assms(1) assms(3) last_in_set less_irrefl list.set_intros(1) lower_bound2_list.elims lower_bound2_split sorted_wrt_append)
+      by (metis "2" assms(1) assms(3) last_in_set less_irrefl list.set_intros(1) lower_bound2.elims lower_bound2_split sorted_wrt_append)
     then show ?case 
       using 2
       by (auto)
   qed
 qed
 
+locale split_range = split_tree split
+  for split::
+    "('a bplustree \<times> 'a::{linorder,order_top,order_bot}) list \<Rightarrow> 'a
+       \<Rightarrow> ('a bplustree \<times> 'a) list \<times> ('a bplustree \<times> 'a) list" +
+  fixes lb2_list ::  "'a \<Rightarrow> ('a::{linorder,order_top,order_bot}) list \<Rightarrow> 'a"
+  assumes lb2_list_req:
+    (* TODO locale that derives such a function from a split function similar to the above *)
+    "sorted_less ks \<Longrightarrow> lb2_list x ks = lower_bound2 x ks"
+begin
+
+fun lb2:: "'a bplustree \<Rightarrow> 'a \<Rightarrow> 'a" where
+  "lb2 (LNode ks) x = (lb2_list x ks)" |
+  "lb2 (Node ts t) x = (
+      case split ts x of (_,(sub,sep)#rs) \<Rightarrow> (
+             lb2 sub x
+      )
+   | (_,[]) \<Rightarrow> lb2 t x
+  )"
+
+text "lower bound 2 proof"
+
+thm lower_bound2_simps
+  (* copied from comment in List_Ins_Del *)
+
+(* lift to split *)
+
+lemma leaves_conc: "leaves (Node (ls@rs) t) = leaves_list ls @ leaves_list rs @ leaves t"
+  apply(induction ls)
+  apply auto
+  done
+
+lemma leaves_split: "split ts x = (ls,rs) \<Longrightarrow> leaves (Node ts t) = leaves_list ls @ leaves_list rs @ leaves t"
+  using leaves_conc split_conc by blast
+
+
+(* Problem: the elements left/right of the separators
+ cannot be excluded from the search for lower_bound2/lower_bound
+and hence we cannot make any guarantees on the quality
+of our result (just that it will be \<le> lower_bound for example)
+
+*)
+
+lemma lb2_sorted_split:
+  assumes "Laligned (Node ts t) u"
+    and "sorted_less (leaves (Node ts t))"
+    and "split ts x = (ls, rs)"
+  shows "lower_bound2 x (leaves (Node ts t)) = lower_bound2 x (leaves_list rs @ leaves t)"
+proof (cases ls)
+  case Nil
+  then have "ts = rs"
+    using assms by (auto dest!: split_conc)
+  then show ?thesis by simp
+next
+  case Cons
+  then obtain ls' sub sep where ls_tail_split: "ls = ls' @ [(sub,sep)]"
+    by (metis list.simps(3) rev_exhaust surj_pair)
+  then have x_sm_sep: "sep < x"
+    using split_req(2)[of ts x ls' sub sep rs]
+    using Laligned_sorted_separators[OF assms(1)]
+    using assms sorted_cons sorted_snoc 
+    by blast
+  moreover have leaves_split: "leaves (Node ts t) = leaves_list ls @ leaves_list rs @ leaves t"
+    using assms(3) leaves_split by blast
+  then show ?thesis
+  proof (cases "leaves_list ls")
+    case Nil
+    then show ?thesis
+      using leaves_split
+      by (metis self_append_conv2)
+  next
+    case Cons
+    then obtain leavesls' l' where leaves_tail_split: "leaves_list ls = leavesls' @ [l']"
+      by (metis list.simps(3) rev_exhaust)
+    then have "l' \<le> sep"
+    proof -
+      have "l' \<in> set (leaves_list ls)"
+        using leaves_tail_split by force
+      then have "l' \<in> set (leaves (Node ls' sub))"
+        using ls_tail_split
+        by auto
+      moreover have "Laligned (Node ls' sub) sep" 
+        using assms split_conc[OF assms(3)] Cons ls_tail_split
+        using Laligned_split_left[of ls' sub sep rs t u]
+        by simp
+      ultimately show ?thesis
+        using Laligned_leaves_inbetween[of "Node ls' sub" sep]
+        by blast
+    qed
+    then have "l' < x"
+      using le_less_trans x_sm_sep by blast
+    then show ?thesis
+      using assms(2) ls_tail_split leaves_tail_split leaves_split x_sm_sep
+      using lower_bound2_split[of "leavesls'" l' "leaves_list rs @ leaves t" x]
+      oops
+
+
+lemma lb2_sorted_split_right:
+  assumes "split ts x = (ls, (sub,sep)#rs)"
+    and "sorted_less (leaves (Node ts t))"
+    and "Laligned (Node ts t) u"
+  shows "lower_bound2 x (leaves_list ((sub,sep)#rs) @ leaves t) = lower_bound2 x (leaves sub)"
+proof -
+  from assms have "x \<le> sep"
+  proof -
+    from assms have "sorted_less (separators ts)"
+      by (meson Laligned_sorted_inorder sorted_cons sorted_inorder_separators sorted_snoc)
+    then show ?thesis
+      using split_req(3)
+      using assms
+      by fastforce
+  qed
+  moreover have leaves_split: "leaves (Node ts t) = leaves_list ls @ leaves sub @ leaves_list rs @ leaves t"
+    using split_conc[OF assms(1)] by auto
+  ultimately show ?thesis
+  proof (cases "leaves_list rs @ leaves t")
+    case Nil
+    then show ?thesis 
+      by (metis assms(1) leaves_split same_append_eq self_append_conv split_range.leaves_split split_range_axioms)
+  next
+    case (Cons r' rs')
+    then have "sep < r'"
+      by (metis (mono_tags, lifting) Laligned_split_right aligned_leaves_inbetween append.right_neutral append_assoc assms(1) assms(3) concat.simps(1) leaves_conc list.set_intros(1) list.simps(8) split_tree.split_conc split_tree_axioms)
+    then have  "x < r'"
+      using \<open>x \<le> sep\<close> by auto
+    moreover have "sorted_less (leaves_list ((sub,sep)#rs) @ leaves t)"
+      using assms sorted_wrt_append split_conc
+      by fastforce
+    ultimately show ?thesis
+      using lower_bound2_split[of "leaves sub" "r'" "rs'" x] Cons 
+      by auto
+  qed
+qed
+
+
+theorem lb2_set_inorder: 
+  assumes "sorted_less (leaves t)"
+    and "aligned l t u"
+  shows "lb2 t x = lower_bound2 x (leaves t)"
+  using assms
+proof(induction t x arbitrary: l u rule: lb2.induct)
+  case (2 ts t x)
+  then obtain ls rs where list_split: "split ts x = (ls, rs)"
+    by (meson surj_pair)
+  then have list_conc: "ts = ls @ rs" 
+    using split_conc by auto
+  show ?case
+  proof (cases rs)
+    case Nil
+    then have "lb2 (Node ts t) x = lb2 t x"
+      by (simp add: list_split)
+    also have "\<dots> = lower_bound2 x (leaves t)"
+      using "2.IH"(1)[of ls rs] list_split Nil
+      using "2.prems" sorted_leaves_induct_last align_last'
+      by metis
+    also have "\<dots> = lower_bound2 x (leaves (Node ts t))"
+      using lower_bound2_split
+      using "2.prems" list_split list_conc Nil
+      sorry
+    finally show ?thesis .
+  next
+    case (Cons a list)
+    then obtain sub sep where a_split: "a = (sub,sep)"
+      by (cases a)
+      then have "lb2 (Node ts t) x = lb2 sub x"
+        using list_split Cons a_split
+        by auto
+      also have "\<dots> = lower_bound2 x (leaves sub)"
+        using "2.IH"(2)[of ls rs "(sub,sep)" list sub sep]
+        using "2.prems" a_split list_conc list_split local.Cons sorted_leaves_induct_subtree
+              align_sub
+        by (metis in_set_conv_decomp)
+      also have "\<dots> = lower_bound2 x (leaves (Node ts t))"
+        using lower_bound2_split
+        using lb2_sorted_split_right "2.prems" list_split Cons a_split
+        using aligned_imp_Laligned sorry
+      finally show ?thesis  .
+    qed
+qed (auto simp add: lb2_list_req)
+
+
+theorem lb2_set_Linorder: 
+  assumes "sorted_less (leaves t)"
+    and "Laligned t u"
+  shows "lb2 t x = lower_bound2 x (leaves t)"
+  using assms
+proof(induction t x arbitrary: u rule: lb2.induct)
+  case (2 ts t x)
+  then obtain ls rs where list_split: "split ts x = (ls, rs)"
+    by (meson surj_pair)
+  then have list_conc: "ts = ls @ rs" 
+    using split_conc by auto
+  show ?case
+  proof (cases rs)
+    case Nil
+    then have "lb2 (Node ts t) x = lb2 t x"
+      by (simp add: list_split)
+    also have "\<dots> = lower_bound2 x (leaves t)"
+      using "2.IH"(1)[of ls rs] list_split Nil
+      using "2.prems" sorted_leaves_induct_last
+      by (metis Lalign_Llast)
+    also have "\<dots> = lower_bound2 x (leaves (Node ts t))"
+      using lower_bound2_split
+      using "2.prems" list_split list_conc Nil
+      sorry
+    finally show ?thesis .
+  next
+    case (Cons a list)
+    then obtain sub sep where a_split: "a = (sub,sep)"
+      by (cases a)
+      then have "lb2 (Node ts t) x = lb2 sub x"
+        using list_split Cons a_split
+        by auto
+      also have "\<dots> = lower_bound2 x (leaves sub)"
+        using "2.IH"(2)[of ls rs "(sub,sep)" list sub sep]
+        using "2.prems" a_split list_conc list_split local.Cons sorted_leaves_induct_subtree
+        by (metis Lalign_Llast Laligned_split_left)
+      also have "\<dots> = lower_bound2 x (leaves (Node ts t))"
+        using lower_bound2_split
+        using lb2_sorted_split_right "2.prems" list_split Cons a_split
+        using aligned_imp_Laligned sorry
+      finally show ?thesis  .
+    qed
+qed (auto simp add: lb2_list_req)
+
+corollary isin_set_Linorder_top: 
+  assumes "sorted_less (leaves t)"
+    and "Laligned t top"
+  shows "lb2 t x = lower_bound2 x (leaves t)"
+  using assms lb2_set_Linorder
+  by simp
+
+end
 
 end
