BPlusTree_ImpRange.thy
@@ -1,0 +1,15 @@
+theory BPlusTree_ImpRange
+imports
+  BPlusTree_Range
+  BPlusTree_Iter
+begin
+
+(* Adding an actual range iterator based on the normal iterator
+is trivial (just forward until we reach the first element \<ge> and stop
+as soon as we have an element <)
+We *could* implement a search for the first element of the range
+however cannot make any (simple) guarantees on its quality
+(see Bplustree_Range to see why *)
+
+
+end
